quickly make everything compile, add hex notation support, add small fib example compiled with riscv64-unknown-elf-gcc toolchain, decode seems to work on it, but running it does not yet work

src/Example.v
@@ -2,48 +2,41 @@ Require Import Coq.Lists.List.
 Import ListNotations.
 Require Import riscv.Riscv.
 Require Import riscv.RiscvBitWidths32.
+Require Import riscv.HexNotation.
+Require Import Coq.ZArith.BinInt.
+Require Import riscv.Memory.
 
+Notation "'Ox' a" := (NToWord _ (hex a)) (at level 50).
 
-Instance NatName: NameWithEq := {| name := nat |}.
-
-Definition var: Set := (@name NatName).
-Definition Reg: Set := (@name NatName).
-
-Definition var_a: var := 0.
-Definition var_b: var := 1.
-Definition var_c: var := 2.
-Definition var_i: var := 3.
-
-(* stores fib(6) into register var_b (inefficient compiler-generated assembly) *)
-Definition fib6_riscv: list Instruction := [
-  Addi (RegS 4) RegO $ (0);
-  Add (RegS var_a) RegO (RegS 4);
-  Addi (RegS 5) RegO $ (1);
-  Add (RegS var_b) RegO (RegS 5);
-  Addi (RegS 6) RegO $ (0);
-  Add (RegS var_i) RegO (RegS 6);
-  Add (RegS 7) RegO (RegS var_i);
-  Addi (RegS 8) RegO $ (6);
-  Sltu (RegS 9) (RegS 7) (RegS 8);
-  Beq (RegS 9) RegO ($ (2) ^* $ (13));
-  Add (RegS 10) RegO (RegS var_a);
-  Add (RegS 11) RegO (RegS var_b);
-  Add (RegS 12) (RegS 10) (RegS 11);
-  Add (RegS var_c) RegO (RegS 12);
-  Add (RegS 13) RegO (RegS var_b);
-  Add (RegS var_a) RegO (RegS 13);
-  Add (RegS 14) RegO (RegS var_c);
-  Add (RegS var_b) RegO (RegS 14);
-  Add (RegS 15) RegO (RegS var_i);
-  Addi (RegS 16) RegO $ (1);
-  Add (RegS 17) (RegS 15) (RegS 16);
-  Add (RegS var_i) RegO (RegS 17);
-  Jal RegO (^~ ($ (2) ^* $ (17)))
+Definition fib6_riscv: list (word 32) := [
+  Ox"00600993";         (* li s3,6 *)
+  Ox"00000a13";         (* li s4,0 *)
+  Ox"00100913";         (* li s2,1 *)
+  Ox"00000493";         (* li s1,0 *)
+  Ox"0140006f";         (* j 101e0 <main+0x44> *)
+  Ox"012a0ab3";         (* add s5,s4,s2 *)
+  Ox"00090a13";         (* mv s4,s2 *)
+  Ox"000a8913";         (* mv s2,s5 *)
+  Ox"00148493";         (* addi s1,s1,1 *)
+  Ox"ff34c8e3"          (* blt s1,s3,101d0 <main+0x34> *)
 ].
 
-Definition initialRiscvMachine(imem: list Instruction): RiscvMachine := {|
-  instructionMem := fun (i: word wXLEN) => nth (Nat.div (wordToNat i) 4) imem InfiniteJal;
-  registers := fun (r: Reg) => $0;
+Notation x0 := (WO~0~0~0~0~0)%word.
+Notation s1 := (WO~0~1~0~0~1)%word.
+Notation s2 := (WO~1~0~0~1~0)%word.
+Notation s3 := (WO~1~0~0~1~1)%word.
+Notation s4 := (WO~1~0~1~0~0)%word.
+Notation s5 := (WO~1~0~1~0~1)%word.
+
+Goal False.
+  set (l := map decode fib6_riscv).
+  cbv in l.
+  (* decoder seems to work :) *)
+Abort.
+
+Definition initialRiscvMachine(imem: list (word 32)): RiscvMachine := {|
+  machineMem := list_to_mem _ imem;
+  registers := fun (r: Register) => $0;
   pc := $0;
   exceptionHandlerAddr := wneg $4;
 |}.
@@ -52,10 +45,12 @@ Definition fib6_L_final(fuel: nat): RiscvMachine :=
   execState (run fuel) (initialRiscvMachine fib6_riscv).
 
 Definition fib6_L_res(fuel: nat): word wXLEN :=
-  (fib6_L_final fuel).(registers) var_b.
+  (fib6_L_final fuel).(registers) s2.
 
 Transparent wlt_dec.
 
 Lemma fib6_res_is_13_by_running_it: exists fuel, fib6_L_res fuel = $13.
-  exists 200. cbv. reflexivity.
-Qed.
+  exists 200%nat.
+  cbv.
+  (* TODO should hold but doesn't *)
+Abort.
