src/Run.v
@@ -1,3 +1,4 @@
+Require Import Coq.ZArith.BinInt.
 Require Import bbv.WordScope.
 Require Import bbv.DepEqNat.
 Require Import riscv.NameWithEq.
@@ -8,61 +9,84 @@ Require Import riscv.Decode.
 Require Import riscv.Program.
 Require Import riscv.Execute.
 Require Import riscv.PowerFunc.
+Require Import riscv.Memory.
 Require Import Coq.Lists.List.
 
 Section Riscv.
 
   Context {B: RiscvBitWidths}.
 
-  Context {Name: NameWithEq}. (* register name *)
-  Notation Reg := (@name Name).
-  Existing Instance eq_name_dec.
+  Definition Register0: Register := $0.
 
   Definition run1{M: Type -> Type}{MM: Monad M}{RVS: RiscvState M}: M unit :=
     pc <- getPC;
-    inst <- loadInst pc;
-    setPC (pc ^+ $4);;
-    execute inst.
+    inst <- loadWord pc;
+    setPC (pc + 4)%Z;;
+    execute (decode inst).
 
   Definition run{M: Type -> Type}{MM: Monad M}{RVS: RiscvState M}: nat -> M unit :=
     fun n => power_func (fun m => run1 ;; m) n (Return tt).
 
   Record RiscvMachine := mkRiscvMachine {
-    instructionMem: word wXLEN -> Instruction;
-    registers: Reg -> word wXLEN;
+    machineMem: mem 32;
+    registers: Register -> word wXLEN;
     pc: word wXLEN;
     exceptionHandlerAddr: word wXLEN;
   }.
 
+  Definition TODO{T: Type}: T. Admitted.
+
   Instance IsRiscvMachine: RiscvState (State RiscvMachine) :=
   {|
       getRegister := fun (reg: Register) =>
-        match reg with
-        | RegO => Return $0
-        | RegS r => machine <- get; Return (machine.(registers) r)
-        end;
+        if dec (reg = Register0) then
+          Return $0
+        else
+          machine <- get; Return (machine.(registers) reg);
+
       setRegister := fun (reg: Register) (v: word wXLEN) =>
-        match reg with
-        | RegO => Return tt
-        | RegS r => machine <- get;
-                    match machine with
-                    | mkRiscvMachine imem regs pc eh =>
-                        put (mkRiscvMachine imem 
-                                            (fun reg2 => if dec (r = reg2) then v else regs reg2)
-                                            pc eh)
-                    end
-        end;
-      loadInst := fun (addr: word wXLEN) =>
-        im <- gets instructionMem;
-        Return (im addr);
-      getPC := gets pc;
-      setPC := fun (newPC: word wXLEN) =>
+        if dec (reg = Register0) then
+          Return tt
+        else
+          machine <- get;
+          match machine with
+          | mkRiscvMachine imem regs pc eh =>
+              put (mkRiscvMachine imem 
+                                  (fun reg2 => if dec (reg = reg2) then v else regs reg2)
+                                  pc eh)
+          end;
+
+      getPC := 
+        p <- gets pc;
+        Return (wordToZ p); (* TODO this should be unsigned *)
+
+      setPC := fun (newPC: Z) =>
         machine <- get;
         match machine with
         | mkRiscvMachine imem regs pc eh =>
-            put (mkRiscvMachine imem regs newPC eh)
+            put (mkRiscvMachine imem regs (ZToWord _ newPC) eh)
         end;
+
+      loadByte := TODO;
+      loadHalf := TODO;
+
+      loadWord := fun x => 
+        m <- gets machineMem;
+        match read_mem (ZToWord 32 (x / 4)) m with
+        | Some v => Return v
+        | None => Return $0
+        end;
+
+      loadDouble := TODO;
+
+      storeByte := TODO;
+      storeHalf := TODO;
+      storeWord := TODO;
+      storeDouble := TODO;
+
   |}.
+
+  Definition InfiniteJal := Jal Register0 (-4).
 
   (* Puts given program at address 0, and makes pc point to beginning of program, i.e. 0.
      TODO maybe later allow any address?
@@ -70,11 +94,10 @@ Section Riscv.
      which might contain any undefined garbage values, so the compiler correctness proof
      will show that the program is correct even then, i.e. no initialisation of the registers
      is needed. *)
-  Definition putProgram(prog: list Instruction)(m: RiscvMachine): RiscvMachine :=
+  Definition putProgram(prog: list (word 32))(m: RiscvMachine): RiscvMachine :=
     match m with
     | mkRiscvMachine _ regs _ eh =>
-        mkRiscvMachine (fun (i: word wXLEN) => nth (Nat.div (wordToNat i) 4) prog InfiniteJal)
-                       regs $0 eh
+        mkRiscvMachine (list_to_mem _ prog) regs $0 eh
     end.
 
 End Riscv.
