src/Memory.v
@@ -1,0 +1,28 @@
+Require Import bbv.Word.
+Require Import riscv.Decidable.
+Require Import Coq.Lists.List.
+
+Section Memory.
+
+  Variable w: nat. (* bit width of addresses and memory words *)
+
+  Definition mem := word w -> option (word w).
+
+  Definition read_mem(x: word w)(m: mem): option (word w) := m x.
+
+  Definition write_mem(x: word w)(v: word w)(m: mem): option (mem) :=
+    match m x with
+    | Some old_value => Some (fun y => if dec (x = y) then Some v else m y)
+    | None => None
+    end.
+
+  Definition no_mem: mem := fun x => None.
+
+  Definition zeros_mem(upTo: word w): mem := fun x => if wlt_dec x upTo then Some $0 else None.
+
+  Definition list_to_mem(l: list (word w)): mem := fun x => nth_error l (wordToNat x).
+
+End Memory.
+
+Arguments read_mem {_} _.
+Arguments write_mem {_} _ _.
